src/Ast/NamesAndLinearForms.dfy
@@ -5,21 +5,25 @@
 
 module NamesAndLinearForms {
   import Ast
+  import Raw = RawAst
 
   export
-    reveals NameAlignment, LinearForm
-    provides LinearFormValues, LinearFormL2R, LinearFormR2L, NewNamePreservesLinearForm
-    provides DistinctConcat
-    provides Ast
+    reveals NameAlignment, LinearForm, HasPrefix
+    provides LinearFormValues, LinearFormL2R, LinearFormR2L, NewNamePreservesLinearForm, NewNamePreservesLinearFormAndIsUnique
+    provides DistinctConcat, PrefixOf, PrefixIsUnique
+    provides Ast, Raw
 
   ghost predicate NameAlignment(xMap: map<string, Ast.NamedDecl>) {
     forall name <- xMap :: xMap[name].Name == name
   }
 
+  // LinearForm(xMap, xs) says that the image of xMap is the set of elements in xs.
   ghost predicate LinearForm<X>(xMap: map<string, X>, xs: seq<X>) {
     (set name <- xMap :: xMap[name]) == set x <- xs
   }
 
+  // Like LinearForm, LinearFormValues(xMap, xs) says that the image of xMap is the set of elements in xs.
+  // but LinearFormValues expresses this property in terms of the map's .Values.
   lemma LinearFormValues<X>(xMap: map<string, X>, xs: seq<X>)
     requires LinearForm(xMap, xs)
     ensures xMap.Values == set x <- xs
@@ -47,13 +51,44 @@ module NamesAndLinearForms {
     name :| name in xMap && xMap[name] == x;
   }
 
-  lemma NewNamePreservesLinearForm(name: string, decl: Ast.NamedDecl, xMap: map<string, Ast.NamedDecl>, xs: seq<Ast.NamedDecl>)
+  lemma NewNamePreservesLinearFormAndIsUnique(name: string, decl: Ast.NamedDecl, xMap: map<string, Ast.NamedDecl>, xs: seq<Ast.NamedDecl>)
     requires NameAlignment(xMap)
     requires LinearForm(xMap, xs)
     requires name !in xMap
     requires decl.Name == name
     ensures forall i :: 0 <= i < |xs| ==> xs[i].Name != name
     ensures LinearForm(xMap[name := decl], xs + [decl])
+  {
+    NewNameIsUnique(name, decl, xMap, xs);
+    NewNamePreservesLinearForm(name, decl, xMap, xs);
+  }
+
+  lemma NewNamePreservesLinearForm<X>(name: string, decl: X, xMap: map<string, X>, xs: seq<X>)
+    requires LinearForm(xMap, xs)
+    requires name !in xMap
+    ensures LinearForm(xMap[name := decl], xs + [decl])
+  {
+    var xMap', xs' := xMap[name := decl], xs + [decl];
+    var n := |xs|;
+    calc {
+      (set xName <- xMap' :: xMap'[xName]);
+      (set xName <- xMap :: xMap'[xName]) + {xMap'[name]};
+      { assert name !in xMap; }
+      (set xName <- xMap :: xMap[xName]) + {decl};
+      { assert LinearForm(xMap, xs); }
+      (set x <- xs) + {decl};
+      { assert xs == xs'[..n] && xs'[n] == decl; }
+      (set x <- xs'[..n]) + {xs'[n]};
+      (set x <- xs');
+    }
+  }
+
+  lemma NewNameIsUnique(name: string, decl: Ast.NamedDecl, xMap: map<string, Ast.NamedDecl>, xs: seq<Ast.NamedDecl>)
+    requires NameAlignment(xMap)
+    requires LinearForm(xMap, xs)
+    requires name !in xMap
+    requires decl.Name == name
+    ensures forall i :: 0 <= i < |xs| ==> xs[i].Name != name
   {
     forall i | 0 <= i < |xs|
       ensures xs[i].Name != name
@@ -70,20 +105,6 @@ module NamesAndLinearForms {
       var xName :| xName in xMap && xMap[xName] == x;
       assert xMap[xName].Name == xName;
       assert xName != name; // since "xName in xMap" and "name !in xMap"
-    }
-
-    var xMap', xs' := xMap[name := decl], xs + [decl];
-    var n := |xs|;
-    calc {
-      (set xName <- xMap' :: xMap'[xName]);
-      (set xName <- xMap :: xMap'[xName]) + {xMap'[name]};
-      { assert name !in xMap; }
-      (set xName <- xMap :: xMap[xName]) + {decl};
-      { assert LinearForm(xMap, xs); }
-      (set x <- xs) + {decl};
-      { assert xs == xs'[..n] && xs'[n] == decl; }
-      (set x <- xs'[..n]) + {xs'[n]};
-      (set x <- xs');
     }
   }
 
@@ -115,5 +136,68 @@ module NamesAndLinearForms {
         }
       }
     }
+  }
+
+  predicate HasPrefix(prefix: string, name: string) {
+    && Raw.LegalVariableName(prefix)
+    && prefix + ".." <= name
+  }
+
+  function PrefixOf(name: string): string
+    requires Raw.HasDoubleDot(name)
+  {
+    var j := FirstDoubleDot(name, 0);
+    name[..j]
+  }
+
+  function FirstDoubleDot(name: string, i: nat): (j: nat)
+    requires i <= |name| && Raw.HasDoubleDot(name[i..])
+    ensures i <= j < |name| - 1 && name[j] == '.' == name[j + 1]
+    ensures forall k :: i <= k < j ==> name[k] != '.' || name[k + 1] != '.'
+    decreases |name| - i
+  {
+    Raw.AboutDoubleDot(name[i..]);
+    ghost var m :| 0 <= m < |name[i..]| - 1 && name[i..][m] == '.' == name[i..][m + 1];
+    assert name[i + m] == '.' == name[i + m + 1];
+    if name[i] == '.' == name[i + 1] then
+      i
+    else
+      assert m != 0;
+      assert 0 <= m - 1 < |name[i + 1..]| - 1 && name[i + 1..][m - 1] == '.' == name[i + 1..][m];
+      Raw.AboutDoubleDot(name[i + 1..]);
+      FirstDoubleDot(name, i + 1)
+  }
+
+  lemma PrefixIsUnique(prefix: string, name: string)
+    requires HasPrefix(prefix, name) && Raw.LegalVariableName(prefix)
+    ensures (Raw.ProveHasDoubleDot(name, |prefix|); PrefixOf(name) == prefix)
+  {
+    var m := |prefix|;
+    assert name[..m] == prefix;
+    assert name[m] == '.' == name[m + 1];
+
+    Raw.ProveHasDoubleDot(name, m);
+    var j := FirstDoubleDot(name, 0);
+    assert PrefixOf(name) == name[..j];
+
+    // From postconditions of FirstDoubleDot:
+    assert 0 <= j < |name| - 1 && name[j] == '.' == name[j + 1];
+    assert forall k :: 0 <= k < j ==> name[k] != '.' || name[k + 1] != '.'; // j is the first double dot
+
+    if
+    case m < j =>
+      // No, j cannot be bigger than m, because there is a double dot at m and j is the first double dot
+      assert false;
+    case j == m - 1 =>
+      // No, because "prefix" is a legal variable name, so it cannot end with a dot
+      reveal Raw.LegalVariableName;
+      assert false;
+    case j < m - 1 =>
+      // No, because "prefix" has no double dot
+      reveal Raw.LegalVariableName;
+      Raw.ProveHasDoubleDot(prefix, j);
+      assert false;
+    case j == m =>
+      // This is the only remain case
   }
 }
