src/Ast/DomainInstantiation.dfy
@@ -1,0 +1,49 @@
+module DomainInstantiation {
+  export
+    provides Instantiate
+    provides Ast, NamesAndLinearForms
+
+  import Basics
+  import Raw = RawAst
+  import opened Ast
+  import NamesAndLinearForms
+
+  method Instantiate(domain: Domain, selfTypeDecl: TypeDecl, typeArguments: seq<Type>) returns (instTypes: seq<TypeDecl>, instFunctions: seq<Function>, instAxioms: seq<Axiom>, instProcedures: seq<Procedure>)
+    requires Raw.LegalVariableName(selfTypeDecl.Name)
+    requires |domain.params| == |typeArguments|
+    requires NamedDecl.Distinct(domain.params + domain.members.types)
+    ensures NamedDecl.Distinct(instTypes)
+    ensures forall typ <- instTypes :: NamesAndLinearForms.HasPrefix(selfTypeDecl.Name, typ.Name)
+  {
+    instTypes, instFunctions, instAxioms, instProcedures := [], [], [], [];
+    var prefix := selfTypeDecl.Name + "..";
+    var typesToBeInstantiated := domain.params + domain.members.types;
+
+    for i := 0 to |typesToBeInstantiated|
+      invariant |instTypes| == i
+      invariant forall j :: 0 <= j < i ==> instTypes[j].Name == prefix + typesToBeInstantiated[j].Name
+    {
+      var typ := typesToBeInstantiated[i];
+      var newName := prefix + typ.Name;
+      var newType := new TypeDecl(newName);
+      instTypes := instTypes + [newType];
+    }
+    // Prove the postconditions about "instTypes"
+    forall i, j | 0 <= i < j < |instTypes|
+      ensures instTypes[i].Name != instTypes[j].Name
+    {
+      Basics.CommonPrefixEquality(prefix, typesToBeInstantiated[i].Name, typesToBeInstantiated[j].Name);
+    }
+    forall i | 0 <= i < |instTypes|
+      ensures NamesAndLinearForms.HasPrefix(selfTypeDecl.Name, instTypes[i].Name)
+    {
+      assert instTypes[i].Name == selfTypeDecl.Name + ".." + typesToBeInstantiated[i].Name;
+      assert selfTypeDecl.Name + ".." <= selfTypeDecl.Name + ".." + typesToBeInstantiated[i].Name;
+    }
+
+    var tMap := map[domain.self := UserType(selfTypeDecl)];
+    for i := 0 to |domain.params| {
+      tMap := tMap[domain.params[i] := typeArguments[i]];
+    }
+  }
+}
